% {\Large \textbf{Mechanical:}}
\qns{First-Order Differential Equation Practice}
\qcontributor{Elena Jia}

\begin{enumerate}

\qitem Solve the equation $\frac{d}{dt} f(t) = 7 f(t) $ given that $f(0) = 3$

\sol{
	This is a basic first-order differential eqution practice. We know the solution of the equation $\frac{d}{dt} f(t) = 7 f(t)$ is in the form $f(t) = A e^{7t}$, as we can check by plugging it into the differential equation. We can find the value of $A$ by using $f(0) = 3$. The final solution is $f(t) = 3 e^{7t}$.
}

\qitem Solve the equation $\frac{d}{dt} f(t) + 5 f(t) = 0 $ given that $f(0) = 2$

\sol{
	$f(t) = 2 e^{-5t}$.
}

\qitem Solve the equation $3 \frac{d}{dt} f(t) + 6 f(t) = 0$ given that $f(0) = 7$

\sol{
	$f(t) = 7 e^{-2t}$.
}

\qitem Solve the equation $\frac{d}{dt} f(t) = 2f(t) + 2 $ given that $f(0) = 3$

\sol{
	To get started on this problem,  we can write the equation as $\frac{d}{dt} f(t) + 1 = 2(f(t) + 1) $. Then we solve for $f(t)+1$ like the previous problems and obtain $f(t)+1 = 4 e^{2t}$. The final solution is $f(t) = 4 e^{2t} - 1$.
}


\qitem Solve the equation $5\frac{d}{dt} f(t) + 3f(t) - 10 = 0 $ given that $f(0) = 8$

\sol{
	$f(t) = \frac{14}{3}e^{\frac{-3}{5} t} + \frac{10}{3}$.
}



\qitem Solve the equation $6\frac{d}{dt} f(t) + 4 = 3f(t) $ given that $f(0) = \frac{1}{3}$

\sol{
	$f(t) = - e^{\frac{1}{2} t} + \frac{4}{3} $.
}


\qitem Solve the equation $3f(t) - 6 f'(t) = 4$ given that $f(2) = \frac{1}{3}$

\sol{
	$f(t) = -e^{\frac{1}{2} t - 1} + \frac{4}{3}$ \\
}

% \qitem  Solve the equation $f'(t) = 5f(t) + 8 e^{5t}$ given that $f(0) = 7$

% \sol{
% 	$7e^{5t}+8e^{5t}t$.
% }


% \qitem  Solve the equation $f'(t) = af(t) + k e^{bt}$

% \sol{
% 	$ce^{at}-\frac{ke^{bt}}{a-b}$.
% }



\end{enumerate}