% {\Large \textbf{Mechanical:}}
\qns{First-Order Differential Equation Practice}


\begin{enumerate}

\qitem Solve the equation $\frac{d}{dt} f(t) = 7 f(t) $ given that $f(0) = 3$

\sol{
	$f(t) = 3 e^{7t}$.
}

\qitem Solve the equation $\frac{d}{dt} f(t) + 5 f(t) = 0 $ given that $f(0) = 2$

\sol{
	$f(t) = 2 e^{-5t}$.
}

\qitem Solve the equation $3 \frac{d}{dt} f(t) + 6 f(t) = 0$ given that $f(0) = 7$

\sol{

	% We know that the solution to the first-order differential equation must be of the form $f(t) = A e^{\lambda t} + B$. If we plug in that definition of $f(t)$ into the given equation, we get
	% \begin{align*}
	% 	3 (A \lambda e^{\lambda t}) + 6(A e^{\lambda t} + B) &= 0 \\
	% 	(3 A \lambda + 6 A)e^{\lambda t} + 6B &= 0
	% \end{align*}
	% We know that the coefficient of the exponential $e^{\lambda t}$ and the constant must be zero, which means that $3A \lambda + 6A = 0$ and $6B = 0$. Solving these yield $\lambda = -2, B = 0$. If we use our initial condition alongside the parameters we just found, we get $7 = f(0) = A e^{-2 (0)} + 0 = A$, implying that $A = 7$. Therefore, 
	$f(t) = 7 e^{-2t}$.
	
}

\qitem Solve the equation $\frac{d}{dt} f(t) = 2f(t) + 2 $ given that $f(0) = 3$

\sol{
	$f(t) = 4 e^{2t} - 1$.
}


\qitem Solve the equation $5\frac{d}{dt} f(t) + 3f(t) - 10 = 0 $ given that $f(0) = 8$

\sol{
	$f(t) = \frac{14}{3}e^{\frac{-3}{5} t} + \frac{10}{3}$.
}



\qitem Solve the equation $6\frac{d}{dt} f(t) + 4 = 3f(t) $ given that $f(0) = \frac{1}{3}$

\sol{
	$f(t) = - e^{\frac{1}{2} t} + \frac{4}{3} $.
}


\qitem Solve the equation $3f(t) - 6 f'(t) = 4$ given that $f(2) = \frac{1}{3}$

\sol{

	% $f(t) = A e^{\lambda t} + B$
	% \begin{align*}
	% 	3 (A e^{\lambda t} + B) - 6(A \lambda e^{\lambda t}) &= 4 \\
	% 	(3A - 6A \lambda) e^{\lambda t} + 3B &= 4 \\
	% 	\lambda &= \frac{1}{2} \\
	% 	B &= \frac{4}{3} \\
	% 	f(t) &= A e^{\frac{1}{2} t} + \frac{4}{3} \\
	% 	f(2) = \frac{1}{3} &= A e^{\frac{1}{2}(2)} + \frac{4}{3} \\
	% 	A &= -\frac{1}{e} \\
	% 	f(t) &= -\frac{1}{e} e^{\frac{1}{2} t} + \frac{4}{3} \\
	% 	&= -e^{\frac{1}{2} t - 1} + \frac{4}{3} \\
	% \end{align*}
	$f(t) = -e^{\frac{1}{2} t - 1} + \frac{4}{3}$ \\
	
}

% \qitem  Solve the equation $f'(t) = 5f(t) + 8 e^{5t}$ given that $f(0) = 7$

% \sol{
% 	$7e^{5t}+8e^{5t}t$.
% }


% \qitem  Solve the equation $f'(t) = af(t) + k e^{bt}$

% \sol{
% 	$ce^{at}-\frac{ke^{bt}}{a-b}$.
% }



\end{enumerate}